theories/L/Complexity/Synthetic.v
@@ -1,170 +1,32 @@
-From Undecidability.L Require Import Tactics.LTactics Computability.Synthetic Prelim.MoreList Prelim.MoreBase Datatypes.LBinNums.
-Require Import CMorphisms.
-From Undecidability.L.Complexity Require Import Monotonic.
-Record inO (f g : nat -> nat) : Type :=
-  {
-    c__inO : nat;
-    n__inO : nat;
-    inO__correct : forall n, n__inO <= n -> f n <= c__inO * g n
-  }.
-
-Arguments inO__correct : clear implicits.
-Arguments inO__correct {_ _}.
-
-Notation " f ∈O g" := (inO f g) (at level 70).
-
-Instance inO_PreOrder : PreOrder inO.
-Proof.
-  split.
-  -exists 1 0. intros. Lia.lia.
-  -intros f g h [c n0 H] [c' n0' H'].
-   exists (c*c') (max n0 n0').
-   intros n Hn.
-   rewrite H,H'. all:Lia.lia.
-Qed.
-
-Record ino (f g : nat -> nat) : Type :=
-  {
-    ino__correct : forall c__ino, 0 < c__ino -> {n__ino | forall n, n__ino <= n -> f n < c__ino * g n}
-  }.
-
-Arguments ino__correct : clear implicits.
-Arguments ino__correct {_ _}.
-
-Notation " f ∈o g" := (ino f g) (at level 70).
-
-Definition n__ino f g (H:f ∈o g) c0 (H' : 0 < c0) : nat := proj1_sig (ino__correct H c0 H').
-
-Definition correct_n__ino f g (H:f ∈o g) c0 (H' : 0 < c0)
-  : forall n, n__ino H H' <= n -> f n < c0 * g n := proj2_sig (ino__correct H c0 H').
-
-Lemma ino_inO_incl f g :
-  f ∈o g -> f ∈O g.
-Proof.
-  intros [H].
-  specialize (H 1 ltac:(Lia.lia)) as (c__ino&H).
-  exists 1 c__ino. intros. apply Nat.lt_le_incl. easy.
-Qed.
+From Undecidability.L Require Import Tactics.LTactics Prelim.MoreList Prelim.MoreBase Datatypes.LBinNums.
+From Undecidability.L.Complexity Require Export Monotonic ONotation.
 
 Inductive is_computable_time {A} {t : TT A} (a : A) fT : Prop :=
-  C : computableTime' a fT -> is_computable_time a fT.
+  C : computableTime a fT -> is_computable_time a fT.
 
 Definition L_decidable_inTime {X} `{R :registered X} (P : X -> Prop) (fT : nat -> nat) :Prop := Eval cbn [timeComplexity] in
   exists f : X -> bool, is_computable_time (t:=TyArr (TyB X) (TyB bool)) f
                                   (fun x _ => (fT (L.size (enc x)),tt)) /\ forall x, P x <-> f x = true.
 
 Definition inTimeO {X} `{R :registered X} P f :=
-  exists f', L_decidable_inTime P f' /\ inhabited (f' ∈O f).
+  exists f', L_decidable_inTime P f' /\ f' ∈O f.
 
 Notation "P ∈TimeO f" := (inTimeO P f) (at level 70).
 
 Definition inTimeo {X} `{R :registered X} P f :=
-  exists f', L_decidable_inTime P f' /\ inhabited (f' ∈o f).
+  exists f', L_decidable_inTime P f' /\ f' ∈o f.
 
 Notation "P ∈Timeo f" := (inTimeo P f) (at level 70).
 
 
 (** Properties *)
 
-
 (** Inclusion *)
 Lemma inTime_mono f g X (_ : registered X):
   f ∈O g -> forall (P : X -> Prop), P ∈TimeO f -> P ∈TimeO g.
 Proof.
-  intros H P [? [? []]]. unfold inTimeO.
-  eexists _. split. 2:constructor.
-  2:setoid_rewrite <- H. all:eassumption.
-Qed.
-
-Lemma inO_add_l f1 f2  g:
-  f1 ∈O g -> f2 ∈O g -> (fun n => f1 n + f2 n) ∈O g.
-Proof.
-  intros [c1 n1 H1] [c2 n2 H2].
-  eexists (c1 + c2) (max n1 n2).
-  intros.
-  rewrite H1,H2.
-  all:Lia.lia.
-Qed.
-
-Require Import CMorphisms.
-Instance inO_pointwise_leq : Proper ( flip (pointwise_relation _ le)  ==> eq ==> Basics.arrow) inO.
-Proof.
-  intros ? ? R1 ? ? <- [c1 n1 H'].
-  eexists c1 n1. hnf in R1. intros. rewrite R1,H'. all:easy.
-Qed.
-
-Lemma inO_mul_c_l c f1  g:
-  f1 ∈O g -> (fun n => c * f1 n) ∈O g.
-Proof.
-  intros [c1 n1 H1].
-  eexists (c1*c) (n1).
-  intros.
-  rewrite H1.
-  all:Lia.lia.
-Qed.
-
-Lemma inO_mul_c_r c f1  g:
-  f1 ∈O g -> (fun n => f1 n * c) ∈O g.
-Proof.
-  intros [c1 n1 H1].
-  eexists (c1*c) (n1).
-  intros.
-  rewrite H1.
-  all:Lia.lia.
-Qed.
-
-Lemma inO_c c n0 f':
-  (forall n', n0 <= n' -> 1 <= f' n') ->  
-  (fun _ => c ) ∈O f'.
-Proof.
-  eexists (c) (n0).
-  intros. rewrite <- H. all:Lia.nia.
-Qed.
-
-Lemma inO_leq n0 f' g:
-  (forall n', n0 <= n' -> f' n' <= g n') ->  
-  f' ∈O g.
-Proof.
-  eexists 1 (n0).
-  intros. rewrite <- H. all:Lia.nia.
-Qed.
-
-Lemma inO_mul_l f1 f2  g1 g2:
-  f1 ∈O g1 -> f2 ∈O g2 -> (fun n => f1 n * f2 n) ∈O (fun n => g1 n * g2 n).
-Proof.
-  intros [c1 n1 H1] [c2 n2 H2].
-  eexists (c1 * c2) (max n1 n2).
-  intros.
-  rewrite H1,H2.
-  all:Lia.lia.
-Qed.
-
-Lemma inO_comp_l f1 f2  g1 g2:
-  f1 ∈O g1 -> f2 ∈O g2 ->
-  monotonic f1 ->
-  (forall x, x <= g2 x ) ->
-  (forall c, (fun x => g1 (c*x)) ∈O g1) -> (fun n => f1 (f2 n)) ∈O (fun n => g1 (g2 n)).
-Proof.
-  intros [c1 n1 H1] [c2 n2 H2] mono2 H' H.
-  specialize (H (c2+n1)) as [c2' n2' H].
-  eexists (c1 * c2') (max (max 1 n2') n2).
-  intros.
-  etransitivity.
-  {hnf in mono2. rewrite mono2. reflexivity. transitivity ((c2+n1)*(g2 n)). 2:reflexivity. rewrite H2. Lia.nia. easy. }
-  specialize (H' n).
-  setoid_rewrite H1. 2:Lia.nia.
-  rewrite H. Lia.nia. Lia.nia.
-Qed.
-  
-(** Only possible with the non-Prop-version of bigO, but not needed in our proofs*)
-Lemma inO__bound f g (H:f ∈O g) : { c0 & forall n, f n <= c0 + c__inO H * g n}.
-Proof.
-  destruct H as [c0 n0 H]. cbn.
-  exists (maxl (map f (natsLess n0))).
-  intros n.
-  decide (n0<=n).
-  -rewrite H. all:Lia.nia.
-  -rewrite (@maxl_leq (f n) (map f (natsLess n0))). Lia.nia. apply in_map_iff. setoid_rewrite natsLess_in_iff. exists n. intuition.          
+  intros H P (?&?&?). unfold inTimeO.
+  eexists _. split. eassumption. now rewrite H1.
 Qed.
 
 (** *** Time Constructibility *)
@@ -180,3 +42,56 @@ Definition timeConstructible_computableTime' f (H:timeConstructible f) :
 
 Definition timeConstructible_inO f (H:timeConstructible f) :
   projT1 H ∈O f := fst (projT2 H).
+
+
+Class computableInO {X Y} `{registered X} `{registered Y} (f:X -> Y) (g: nat -> nat) : Type:=
+  {
+    fT_inO : nat -> nat;
+    compO : computableTime' f (fun x _ => (fT_inO (size (enc x)),tt));
+    lin_t__enc : fT_inO ∈O g;
+    mono_t__enc : monotonic fT_inO;
+  }.
+
+Smpl Add (simple apply mono_t__enc) : monotonic.
+
+Lemma smpl_fT_inO X Y `{registered X} `{registered Y} (f: X -> Y) (g:nat -> nat) {H':computableInO f g} h:
+  g ∈O h -> (fT_inO ∈O h).
+Proof.
+  intros <-. apply lin_t__enc. 
+Qed.
+
+Smpl Add simple eapply smpl_fT_inO : inO.
+
+
+
+Lemma smpl_inOPoly_fT_inO X Y `{registered X} `{registered Y} (f: X -> Y) (g:nat -> nat) {H':computableInO f g}:
+  inOPoly g -> inOPoly fT_inO.
+Proof.
+  intros. now rewrite lin_t__enc.
+Qed.
+
+Lemma inOPoly_computable (f:nat -> nat):
+  inOPoly f -> exists (f':nat -> nat) f__T, is_computable_time (t:=TyArr _ _) f' (fun n _ => (f__T n,tt)) /\ inOPoly f__T /\ (forall x, f x <= f' x) /\ inOPoly f' /\ monotonic f' /\ monotonic f__T.
+Proof.
+  intros (i&Hf).
+  eapply inO__bound in Hf as (c&Hf).
+  exists (fun n => c + c*n^i),(fun n => 19 * i * n + 11 * i * n ^ i + 19 * i + 11 * n ^ i * c + 30 * c + 29).
+  split;split. 3:split;[easy|repeat split].
+  1:{ extract. solverec. }
+  all:smpl_inO.
+  all: eexists i; easy.
+Qed.
+
+
+Smpl Add 12 simple eapply smpl_inOPoly_fT_inO : inO.
+
+
+Record polyTimeComputable X Y `{registered X} `{registered Y} (f : X -> Y): Prop :=
+  {
+    polyTimeC__t : nat -> nat;
+    polyTimeC__comp : is_computable_time (t:=TyArr _ _) f (fun x _ => (polyTimeC__t (L.size (enc x)),tt));
+    polyTimeC__polyTime : inOPoly polyTimeC__t ;
+    polyTimeC__mono : monotonic polyTimeC__t;
+    polyTimeC__polyRes : exists f', (forall x, size (enc (f x))
+                                             <= f' (size (enc x)) ) /\ inOPoly f' /\ monotonic f'
+  }.
