theories/L/Complexity/TimeHierarchyTheorem.v
@@ -1,340 +1,12 @@
-From Undecidability.L Require Import L Tactics.LTactics.
+From Undecidability.L Require Import L Tactics.LTactics AbstractMachines.LargestVar.
 
-From Undecidability.L.AbstractMachines Require Import AbstractHeapMachineDef UnfoldTailRec FunctionalDefinitions.
-From Undecidability.L.AbstractMachines.Computable Require Import Unfolding HeapMachine Shared.
+From Undecidability.L Require Import AbstractHeapMachineDef UnfoldTailRec AbstractHeapMachine.
+From Undecidability.L.AbstractMachines.Computable Require Import Unfolding HeapMachine Shared EvalForTime EvalForTimeBool.
 
 From Undecidability.L.Complexity Require Import Synthetic AbstractTimeHierarchyTheorem.
 
 From Undecidability.L.Datatypes Require Import Lists LBinNums.
 From Undecidability.L.Functions Require Import BinNums BinNumsCompare UnboundIteration.
-
-
-(*Require Import LNat LBool LBinNums LTactics Complexity.Synthetic LProd Functions.BinNumsCompare.
-Require Import AbstractHeapMachine AbstractMachines.FunctionalDefinitions Programs.
-Require Import Equality Eval.
-Require Import Functions.UnboundIteration Functions.BinNums.
-
-From L.Functions Require Import Size Proc.
-
-Require Import AbstractMachines.Computable.Shared HeapMachine Unfolding Programs AbstractMachines.Computable.Compile AbstractMachines.LargestVar ARS.
-*)
-Section E.
-
-  Definition extractRes (sigma : list AbstractHeapMachineDef.task * list clos * list heapEntry) :=
-    match sigma with
-      ([],[g],_) => Some (g)
-    | _ => None
-    end.
-
-  Definition E__step '(i,sigma) : _ + bool:=
-    let '(_,_,H):= sigma in
-    match extractRes sigma with
-      Some g => match unfoldBoolean H g with
-                Some false => inr false
-              | _ => inr true
-              end
-    | _ => if (0 <? i)%N then 
-            match heapStep sigma with
-              Some sigma' => inl (N.pred i,sigma')
-            | _ => inr true
-            end
-          else inr true
-    end.
-
-  Definition time_E__step x :=
-    let '(i,x) := x in
-    let '(T,V,H):=x in
-    match extractRes x with
-      Some g  => unfoldBool_time (length H) (Init.Nat.max (largestVarH H) (largestVarC g))
-    | _ => N.size_nat i * 12
-            + if (0 <? i)%N
-              then heapStep_time T H
-              else 0
-    end + 81.
-
-  Lemma spec_extractRes sigma:
-    match extractRes sigma with
-      Some g => exists H, sigma = ([],[g],H)
-    | None => forall g H, sigma <> ([],[g],H)
-    end.
-  Proof.
-    unfold extractRes.
-    all:repeat (let eq := fresh "eq" in destruct _ eqn:eq).
-    all:try congruence. eexists _;repeat f_equal. congruence.
-  Qed.
-
-  Arguments extractRes : simpl never.
-  
-  Lemma spec_E__step i sigma:
-    match E__step (i,sigma) with
-      inl (i',sigma') => i = N.succ i' /\ step sigma sigma' /\ extractRes sigma = None
-    | inr b =>
-      match extractRes sigma with
-        None => b = true /\ (i = 0%N \/ terminal step sigma)
-      | Some g => b = false <-> unfoldBoolean (snd sigma) g = Some false
-      end
-    end.
-  Proof.
-    specialize (heapStep_sound sigma) as R.
-    specialize (spec_extractRes sigma) as H''.
-    all:cbn.
-    all:destruct sigma as [[T V] H];cbn [snd].
-    all:destruct (N.ltb_spec0 0 i);[|replace i with (0%N) by Lia.nia].
-    all:repeat (let eq := fresh "eq" in destruct _ eqn:eq).
-    all:try discriminate.
-    all:subst.
-    all:repeat match goal with
-                 H :  inl _ = inl _ |- _ => inv H
-               | H :  inr _ = inr _ |- _ => inv H
-end.
-    1:now split;(tauto + Lia.nia).
-    all:try easy.
-    all:left.
-    all:repeat esplit.
-    all:congruence.
-  Qed.
-  
-  Instance termT_extractRes : computableTime' extractRes (fun _ _ => (23,tt)).
-  Proof.
-  extract. solverec. 
-  Qed.
-  
-  Instance termT_E__step : computableTime' E__step (fun x _ => (time_E__step x,tt)).
-  Proof. 
-    extract. intros (i&((T&V)&H)). unfold time_E__step. (*recRel_prettify2.*)
-    all:solverec.
-   Qed. 
-
-  Arguments E__step : simpl never.
-  (*
-  Lemma time_E__step_eq i T V H:
-    ~(T=[] /\ exists g, V=[g]) ->
-    time_E__step (i, (T, V, H))
-    = N.size_nat i * 12
-      + (if (0 <? i)%N then heapStep_time T H else 0)
-      + 60.
-  Proof.
-    intros ?.
-    unfold time_E__step. destruct T. destruct V as [|? []]. 2:exfalso.
-    all:destruct (N.ltb_spec0 0 i);[|try easy]. all:easy.
-  Qed.*)
-  
-  
-  Definition init__E (fuel:N) (s:term) :=
-    ((4 * fuel +1)%N,init s).
-
-  Instance termT_init__E : computableTime' init__E (fun fuel (_:unit) => (1,fun s (_:unit) => (size s * 108 + N.size_nat fuel * 84 + 259,tt))).
-  Proof.
-    eapply computableTimeExt with (x:=fun fuel s => ((fuel + fuel + fuel + fuel +1)%N,init s)).
-    -unfold init__E. repeat intro. hnf. f_equal. Lia.nia.
-    -extract.
-    recRel_prettify2. reflexivity.
-    change (N.size_nat 1) with 1. ring_simplify.
-    
-    repeat rewrite N_size_nat_add_leq.
-    rewrite !Nat.max_l. all:try Lia.lia.
-  Qed.
-
-  Tactic Notation "destruct" "*" "eqn" :=
-    let E := fresh "eq" in destruct * eqn:E.
-
-  Definition R__step := fun '(i,s) '(i',s') => i = N.succ i' /\ step s s'.
-
-  Lemma pow_Rstep k i i' x x':
-    ARS.pow R__step k (i,x) (i',x')
-    -> i'= (i - N.of_nat k)%N /\ ARS.pow step k x x'.
-  Proof.
-    intros R.
-    induction k in i',x',R|-*.
-    {inv R. split. Lia.lia. reflexivity. }
-    replace (S k) with (k + 1) in * by omega.
-    eapply pow_add in R as ((i''&x'')&R&R'').
-    eapply IHk in R as (->&R). eapply rcomp_1 in R'' as [? R''].
-    split. Lia.nia. eapply pow_add;eexists. split. eauto. now eapply rcomp_1 with (R:=step).
-  Qed.
-  Import Undecidability.L.AbstractMachines.LargestVar Undecidability.L.AbstractMachines.AbstractHeapMachine.
-  Lemma time_uiter_E__step s fuel:
-    closed s ->
-    uiterTime E__step (fun x (_:unit) => (time_E__step x,tt)) (N.to_nat fuel + 1) (fuel,init s) <=
-    (N.to_nat fuel + 1) * (N.size_nat fuel * 12 + heapStep_timeBound (largestVar s) (N.to_nat fuel) + 90) + (unfoldBool_time (N.to_nat fuel) (largestVar s)).
-  Proof.
-    intros cs.
-    rewrite uiterTime_computesRel
-      with (R:= R__step)
-           (t__step := N.size_nat fuel * 12 + heapStep_timeBound (largestVar s) (N.to_nat fuel) + 81)
-           (t__end := (unfoldBool_time (N.to_nat fuel) (largestVar s))).
-    2:{
-      intros k' (i'&x') ? R.
-      eapply pow_Rstep in R as (->&R). cbn [fst].
-      specialize spec_E__step with (i:=(fuel - N.of_nat k')%N) (sigma:=x') as H'.
-      specialize (spec_extractRes x') as Hx'.
-      -destruct x' as [[T V] Hp].
-       cbn [fst snd] in *.
-       unfold time_E__step.
-       destruct extractRes.
-       +destruct E__step as [[]|]. now destruct H'. split. 2:tauto.
-        rewrite unfoldBool_time_mono with (l':=(N.to_nat fuel)) (n':=(largestVar s)).
-        *now omega.
-        *rewrite length_H. 2:eassumption. Lia.nia.
-        *eapply subterm_property in R as (_&H__V&H__H).
-          eapply Nat.max_case.
-         --eapply largestVarH_bound.
-           intros [] ? ?. cbn.
-           eapply subterm_largestVar.
-           apply H__H in H0.
-           eapply subterm_lam_inv in H0. easy.
-         --destruct Hx' as (?&[= -> -> <-]).
-           destruct p.
-           eapply subterm_largestVar.
-           eapply subterm_lam_inv. eauto.
-       +split.
-        *rewrite N_size_nat_monotone with (n':=fuel). 2:Lia.nia.
-         destruct N.ltb_spec0 with (x:=0%N) (y:=(fuel - N.of_nat k')%N). 2:Lia.nia.
-         rewrite heapStep_timeBound_le. 2:eassumption.
-         rewrite heapStep_timeBound_mono with (k':=N.to_nat fuel). 2:Lia.nia. Lia.nia.
-        *destruct E__step as [[]|]. 2:easy.
-         split. 2:easy. easy.
-    }
-    Lia.nia.
-  Qed.  
-  
-  Lemma sound_E__step fuel x: {b & loopSum (N.to_nat fuel +1 ) E__step (fuel,x) = Some b}.
-  Proof.
-    remember (N.to_nat fuel) as n eqn:eqn.
-    induction n in eqn,fuel,x|-*.
-    all:cbn.
-    all:specialize (spec_E__step fuel x) as H'.
-    all:destruct E__step as [[]|].
-    1:exfalso;Lia.nia.
-    1,3:eauto.
-    {destruct H' as (->&?&?).
-     edestruct IHn with (fuel:=n0). Lia.nia.
-     eauto.
-    }
-  Qed.      
-
-  Definition E : term := Eval cbn [convert TH]in (λ fuel s, !!(uiter E__step) (!!(extT (init__E)) fuel s)).
-
-  Definition t__E maxVar (size:nat) fuel :=
-    let fuel' := (4*fuel + 1) in
-    size *108 + N.size_nat (N.of_nat fuel) * 84+
-    unfoldBool_time fuel' maxVar + (fuel' + 1) * (N.size_nat (N.of_nat fuel') * 12
-                                                        + heapStep_timeBound maxVar fuel' +90) +262.
-
-  
-  Lemma sound_E__step2' i sigma b:
-    loopSum (N.to_nat i + 1) E__step (i,sigma) = Some b
-    -> reflect (exists k g H, k <= N.to_nat i /\ ARS.pow step k sigma ([],[g],H) /\ unfoldBoolean H g = Some false) (negb b).
-  Proof.
-    intros H.
-    eapply iff_reflect.
-    eapply loopSum_rel_correct2 with (R:=R__step) in H as (k&(x'&i')&?&eq1&R&Ter&eq2).
-    2:{ clear i H. intros [i x]. assert (H':=spec_E__step i x).
-        destruct E__step as [[]|b'].
-        +destruct H' as (->&?&?).
-         hnf. easy.
-        +intros [i' x'] R'. destruct R' as (->&R').
-         assert  (Hx:=spec_extractRes x). destruct extractRes.
-        -destruct Hx as (?&->).
-         inv R'.
-        -destruct H' as (->&[|Ter]). easy.
-         edestruct Ter. easy.
-    }
-    eapply pow_Rstep in R as (->&R).
-    eassert (H'':=spec_E__step _ _ ).
-    unfold state in *.
-    rewrite eq2 in H''.
-    eassert (H':=spec_extractRes i').
-    split;destruct b;cbn;try congruence.
-    -intros (k'&g&Hp&?&?&?). exfalso.
-     edestruct uniform_confluence_parameterized_terminal
-       with (3:=H1) (4:=R) as (n'&R'&eq').
-     { eapply functional_uc, step_functional. }
-     { intros ? Ht. inv Ht. }
-     destruct extractRes.
-     +destruct H' as (?&->). destruct n'. now inv R'. destruct R' as (?&R''&?). inv R''.
-     +replace n' with 0 in *.
-      2:{
-        destruct H'' as (_&[]). Lia.nia.
-        destruct n'. easy. destruct R' as (?&R'&?). now edestruct H3.
-      }
-      inv R'. eapply H'. easy.
-    -intros _.
-     destruct extractRes. 2:easy.
-     destruct H' as (?&->).
-     firstorder.
-  Qed.
-  
-  Lemma E__spec (s:term) (fuel : N):
-    closed s ->
-    exists res : bool,
-      E (enc fuel) (enc s) ⇓(<=t__E (largestVar s) (size s) (N.to_nat fuel)) (enc res) /\
-      if res
-      then ~ (s ⇓(<= N.to_nat fuel ) (enc false))
-      else s ⇓(<= N.to_nat fuel) (enc false).
-  Proof.
-    intros cs.
-    unfold E.
-    edestruct sound_E__step as [b ?].
-    exists b.
-    split.
-    -eapply le_evalLe_proper.
-     2-3:reflexivity.
-     2:{ Lsimpl.
-         eapply uiter_sound.
-         eapply e.
-     }
-     unfold init__E.
-     pose (fuel':=(4*fuel + 1)%N).
-     fold fuel'.
-     recRel_prettify2.
-     erewrite time_uiter_E__step. 2:easy.
-     unfold t__E.
-     replace (4 * N.to_nat fuel + 1) with (N.to_nat fuel') by (unfold fuel';Lia.lia).
-     rewrite !Nnat.N2Nat.id.
-     Lia.nia.
-    -pose (fuel':=(4*fuel + 1)%N).
-     fold fuel' in e.
-     eapply sound_E__step2' in e.
-     destruct b;inv e.
-     +intros (k'&Hle&R)%evalLe_evalIn.
-      eapply ResourceMeasures.timeBS_evalIn in R.
-      eapply correctTime in R as (?&?&?&?). 2:easy.
-      apply H.
-      do 3 eexists. split;[|split]. 2:now eauto. subst fuel'. Lia.nia.
-      eapply unfoldBoolean_complete. easy.
-     +destruct H as (k&g&H&Hleq&R&rep).      
-      edestruct soundness as (g'&H'&t&n&eq'&EV&rep'&eqk).
-      { eassumption. }
-      { split. easy. intros ? R'. inv R'. }
-      revert eq'. intros [= <- <-].
-      eapply unfoldBoolean_sound in rep.
-      specialize (reprC_functional rep rep') as <-.
-      subst fuel'.
-     
-      eapply evalIn_evalLe.
-      2:{ eapply ResourceMeasures.timeBS_evalIn. eassumption. }
-      Lia.lia.
-  Qed.
-
-  Lemma mono_t__E maxVar maxVar' x x' size size' :
-    maxVar <= maxVar' -> x <= x' -> size <= size' -> t__E maxVar size x <= t__E maxVar' size' x'.
-  Proof.
-    intros H1 H2 H3.
-    unfold t__E.
-    repeat (lazymatch goal with
-              |- _ + _ <= _ + _ => eapply plus_le_compat
-            | |- _ * _ <= _ * _ => eapply mult_le_compat
-            | |- _ => first [eassumption | reflexivity | eapply N_size_nat_monotone | eapply unfoldBool_time_mono | Lia.nia |eapply heapStep_timeBound_mono'] 
-            end).
-  Qed.
-
-  Lemma suplin_t__E maxVar size x : x <= t__E maxVar size x. 
-  Proof.
-    unfold t__E. Lia.nia.
-  Qed.
-End E.
-
 
 Section TimeHierarchy.
 
@@ -346,69 +18,100 @@ Section TimeHierarchy.
   Check timeConstructible_inO TC__f.
   Definition comp_t__E: computableTime' (fun n => N.of_nat (f n)) (fun n _ => (fT n,tt)) := timeConstructible_computableTime' TC__f.
   Definition inO_time_t__E: fT ∈O f := timeConstructible_inO TC__f.
-
-
-  Let start (w : term * nat) : term :=
-    let '(s,padding) := w in (s (enc w)).
-
-  Lemma E__proc : proc E.
-  Proof.
-    unfold E. Lproc.
-  Qed.
   
   Definition L__f : term * nat -> Prop :=
     Eval unfold L__f in
       @L__f f.
+
+
+  Definition E (fuel:N) (s:term) := negb (evalForTimeBool false fuel s).
+                                      
+  
+  Instance term_t__E : computableTime' E (fun fuel _ => (1, fun s _ => (t__evalForTimeBool (largestVar s) (size s) (N.to_nat fuel) + 7, tt))).
+  Proof.
+    extract. solverec.
+  Qed.
+
+  Definition t__E (largestVar size:nat) fuel := t__evalForTimeBool largestVar size fuel + 8.
+
+  
+  
+  Lemma E__spec (s:term) (fuel : N):
+      closed s ->
+      exists res : bool,
+        (extT E) (enc fuel) (enc s) ⇓(<=t__E (largestVar s) (size s) (N.to_nat fuel)) (enc res) /\
+        if res
+        then ~ (s ⇓(<= N.to_nat fuel ) (enc false))
+        else s ⇓(<= N.to_nat fuel) (enc false).
+  Proof.
+    intros. eexists. split.
+    {
+      eapply le_evalLe_proper, evalLe_trans. 2,3:reflexivity.
+      2:now Lsimpl.
+      2:Lreflexivity.
+      solverec. reflexivity.
+    }
+    unfold E. destruct (evalForTimeBool_spec false s fuel).
+    -cbn. easy.
+    -cbn. easy.
+  Qed.
+  
+  Lemma mono_t__E maxVar maxVar' x x' size size' :
+    maxVar <= maxVar' -> x <= x' -> size <= size' -> t__E maxVar size x <= t__E maxVar' size' x'.
+  Proof.
+    intros H1 H2 H3.
+    unfold t__E,t__evalForTimeBool.
+    rewrite mono_t__evalForTime. 2-4:eassumption.
+    repeat (lazymatch goal with
+              |- _ + _ <= _ + _ => eapply plus_le_compat
+            | |- _ * _ <= _ * _ => eapply mult_le_compat
+            | |- _ => first [eassumption | reflexivity | eapply N_size_nat_monotone | eapply unfoldBool_time_mono | Lia.nia |eapply heapStep_timeBound_mono'] 
+            end).
+  Qed.
+
+  Lemma suplin_t__E maxVar size x : x <= t__E maxVar size x. 
+  Proof.
+    unfold t__E,t__evalForTimeBool . intros. rewrite <- suplin_t__evalForTime. Lia.nia.
+  Qed.
   
   Lemma inO_size_nat f' g:
     f' ∈O g ->
     (fun n => N.size_nat (N.of_nat (f' n))) ∈O g.
   Proof.
-    intros [c0 n0 H].
-    eexists c0 n0.
+    intros (c0&n0&H).
+    eexists c0,n0.
     intros. rewrite N_size_nat_leq. easy.
   Qed.
 
-  Ltac inO_leq n := simple eapply inO_leq with (n0:=n);intros ? ?;try rewrite <- !f_geq_n;Lia.nia.
-
-  Ltac inO_safe := once (lazymatch goal with
-                           |- (fun n => _ * _ ) ∈O _ =>
-                           first [simple eapply inO_mul_c_l
-                                 | simple eapply inO_mul_c_r]
-                         | |- _ =>
-                           first [simple eapply inO_add_l 
-                                 | simple eapply inO_mul_c_l
-                                 | simple eapply inO_mul_c_r
-                                 | simple eapply inO_c with (n0:=1);intro;try rewrite <- !f_geq_n;Lia.nia
-                                 | inO_leq 1]
-                         end).
-
+  Ltac inO_leq n := simple eapply inO_leq with (n0:=n);intros ;try rewrite <- !f_geq_n;nia.
   
   Lemma in_O_t__E :
     (fun n : nat => t__E n (2 * n) (f n)) ∈O (fun n => n * f n * f n).
   Proof.
-    unfold t__E.
-    repeat inO_safe.
+    unfold t__E,t__evalForTimeBool,t__evalForTime.
+
+    all:unfold unfoldBool_time.
+    all:unfold heapStep_timeBound,Lookup.lookupTime.
+    smpl_inO.
+    1,4,6-9:inO_leq 1.
     2:unfold unfoldBool_time.
-    2-3:unfold heapStep_timeBound,Lookup.lookupTime.
-    
-    -eapply inO_size_nat. repeat inO_safe.
-    -repeat inO_safe.
-     simple eapply inO_mul_l.
-     all:repeat inO_safe.
+    2-3:unfold heapStep_timeBound,Lookup.lookupTime.     
+    -eapply inO_size_nat. inO_leq 1.
     -transitivity (fun n => f n * ( n * f n)). 2:inO_leq 1.
      simple eapply inO_mul_l.
-     all:repeat inO_safe.
-     +eapply inO_size_nat. repeat inO_safe.
-     +simple eapply inO_mul_l.
-      all:repeat inO_safe.
+     all:smpl_inO.
+     1-2,5-8:solve [inO_leq 1].
+     +eapply inO_size_nat. smpl_inO. all:inO_leq 1.
+     +simple eapply inO_mul_l. all:smpl_inO. all:inO_leq 1.
+    -setoid_rewrite Nat.mul_comm at 1. eapply inO_mul_l.
+     all:smpl_inO. all:try inO_leq 1.
   Qed.
   
   Lemma LA_In_f_times_step':
     L__f ∈TimeO (fun n : nat => t__E n (2 * n) (f n)).
   Proof.
     eapply LA_In_f_times_step.
-    all:eauto using comp_t__E,E__spec,E__proc,inO_time_t__E,mono_t__E,suplin_t__E.
+    all:eauto using comp_t__E,E__spec,proc_extT,inO_time_t__E,mono_t__E,suplin_t__E.
   Qed.
   
   Lemma L_A_notIn_f : ~ L__f ∈Timeo f.
@@ -431,5 +134,7 @@ Section TimeHierarchy.
   Qed.
 End TimeHierarchy.
 
-Check TimeHierarchyTheorem.
+(**Check TimeHierarchyTheorem.
+Axiom free: 
 Print Assumptions TimeHierarchyTheorem.
+*)
