theories/L/Complexity/LinTimeDecodable.v
@@ -1,0 +1,74 @@
+From Undecidability.L.Tactics Require Import LTactics.
+From Undecidability.L.Datatypes Require Import LNat Lists LTerm LOptions.
+
+From Undecidability.L Require Import Functions.Decoding Complexity.Synthetic.
+
+Class linTimeDecodable `(X:Type) `{decodable X}: Type :=
+  {
+    c__linDec : nat;
+    comp_enc_lin : computableTime' (decode X) (fun x _ => (size x *c__linDec + c__linDec,tt));
+  }.
+
+Arguments linTimeDecodable : clear implicits.
+Arguments linTimeDecodable _ {_ _}.
+
+Arguments c__linDec : clear implicits.
+Arguments c__linDec _ {_ _ _}.
+
+Existing Instance comp_enc_lin.
+
+Lemma linDec_polyTimeComputable  X `{_:linTimeDecodable X}: polyTimeComputable (decode X).
+Proof.
+  evar (f:nat -> nat).
+  exists f.
+  -split. eexists _. 
+   eapply computesTime_timeLeq.
+   2:now eapply comp_enc_lin.
+   intros x _;cbn [fst snd]. split.
+   2:easy.
+   rewrite size_term_enc_r. generalize (size (enc x)) as n;intros.
+   [f]:intro. unfold f. reflexivity.
+  -unfold f. smpl_inO.
+  -unfold f. smpl_inO.
+  -evar (f':nat -> nat).
+   exists f'. 
+   repeat eapply conj.
+   +intros t.
+    specialize (decode_correct2 (X:=X) (t:=t)) as H'.
+    destruct decode.
+    setoid_rewrite <- H'. 2:reflexivity.
+    *rewrite size_option,LTerm.size_term_enc_r.
+    generalize (size (enc (enc x))). [f']:intro. unfold f'. reflexivity.
+    *unfold enc at 1. cbn. unfold f'. easy.
+   +unfold f'. smpl_inO.
+   +unfold f'. smpl_inO.
+Qed.
+
+Instance linDec_nat : linTimeDecodable nat.
+Proof.
+  evar (c:nat). exists c.
+  unfold decode,decode_nat;cbn. extract.
+  recRel_prettify2;cbn[size];ring_simplify.
+  [c]:exact 9.
+  all:unfold c;try lia.
+Qed.
+
+Instance linDec_term : linTimeDecodable term.
+Proof.
+  evar (c:nat). exists c.
+  unfold decode,decode_term;cbn. extract.
+  recRel_prettify2;cbn[size];ring_simplify.
+  [c]:exact (max (c__linDec nat) 10).
+  all:unfold c;try nia.
+Qed.
+
+Instance linDec_list X `{_:linTimeDecodable X}: linTimeDecodable (list X).
+Proof.
+  evar (c:nat). exists c.
+  unfold decode,decode_list,list_decode;cbn.
+  extract.
+  recRel_prettify2;cbn[size];ring_simplify.
+  [c]:exact (max (c__linDec X) 12).
+  all:unfold c;try nia.
+Qed.
+
