theories/L/Complexity/Monotonic.v
@@ -1,5 +1,56 @@
-
+From smpl Require Import Smpl.
+From Undecidability Require Import L.Prelim.MoreBase.
 Definition monotonic (f:nat -> nat) : Prop :=
   forall x x', x <= x' -> f x <= f x'.
 
-Hint Unfold monotonic : typeclass_instances.
+Lemma monotonic_c c: monotonic (fun _ => c).
+Proof.
+  hnf.
+  intros **. easy.
+Qed.
+
+
+Lemma monotonic_add f1 f2: monotonic f1 -> monotonic f2 -> monotonic (fun x => f1 x + f2 x).
+Proof.
+  unfold monotonic.
+  intros H1 H2 **.
+  rewrite H1,H2. reflexivity. all:eassumption.
+Qed.
+
+Lemma monotonic_mul f1 f2: monotonic f1 -> monotonic f2 -> monotonic (fun x => f1 x * f2 x).
+Proof.
+  unfold monotonic.
+  intros H1 H2 **.
+  rewrite H1,H2. reflexivity. all:eassumption.
+Qed.
+
+Require Import Nat.
+Lemma monotonic_pow_c f1 c: monotonic f1  -> monotonic (fun x => (f1 x) ^ c).
+Proof.
+  intros **. 
+  unfold monotonic.
+  intros H1 **. eapply PeanoNat.Nat.pow_le_mono_l. apply H. easy.
+Qed.
+
+Lemma monotonic_x: monotonic (fun x => x).
+Proof.
+  unfold monotonic. easy.
+Qed.
+
+Lemma monotonic_comp f1 f2: monotonic f1 -> monotonic f2 -> monotonic (fun x => f1 (f2 x)).
+Proof.
+  unfold monotonic.
+  intros H1 H2 **.
+  rewrite H1. reflexivity. eauto.
+Qed.
+
+Smpl Create monotonic.
+Smpl Add 10 (first [ simple eapply monotonic_add | simple eapply monotonic_mul | simple eapply monotonic_c | simple eapply monotonic_x | simple eapply monotonic_pow_c] )  : monotonic.
+
+Smpl Add 20 (lazymatch goal with
+               |- monotonic (fun x => ?f (@?g x)) =>
+               (lazymatch g with
+               | fun x => x => fail
+               | _ => simple eapply monotonic_comp
+               end)
+             end) : monotonic.
