theories/L/Complexity/ONotation.v
@@ -1,0 +1,227 @@
+From Undecidability Require Import Shared.Prelim L.Prelim.MoreBase L.Complexity.Monotonic.
+Require Import smpl.Smpl.
+Require Import Nat Lia.
+
+(** ** O notation *)
+
+Definition inO (f g : nat -> nat) : Prop := exists c n0, forall n, n0 <= n -> f n <= c * g n.
+
+Notation " f ∈O g" := (inO f g) (at level 70).
+
+Instance inO_PreOrder : PreOrder inO.
+Proof.
+  split.
+  -exists 1,0. intros. Lia.lia.
+  -intros f g h (c&n0&H) (c'&n0'&H').
+   exists (c*c'),(max n0 n0').
+   intros n Hn.
+   rewrite H,H'. all:Lia.lia.
+Qed.
+
+
+Instance inO_pointwise_leq : Proper ( Basics.flip (pointwise_relation _ le)  ==> eq ==> Basics.impl) inO.
+Proof.
+  intros ? ? R1 ? ? <- (c1&n1&H').
+  eexists c1,n1. hnf in R1. intros. rewrite R1,H'. all:easy.
+Qed.
+
+Instance inO_pointwise_le : Proper ((pointwise_relation _ eq) ==> eq ==> Basics.impl) inO.
+Proof.
+  intros ? ? R1 ? ? <-. hnf in R1.
+  eapply inO_pointwise_leq. 2:easy. hnf. intros. rewrite R1. easy.
+Qed.
+
+
+Lemma inO_add_l f1 f2  g:
+  f1 ∈O g -> f2 ∈O g -> (fun n => f1 n + f2 n) ∈O g.
+Proof.
+  intros (c1&n1&H1) (c2&n2&H2).
+  eexists (c1 + c2),(max n1 n2).
+  intros.
+  rewrite H1,H2.
+  all:Lia.lia.
+Qed.
+
+Lemma inO_mul_c_l c f1  g:
+  f1 ∈O g -> (fun n => c * f1 n) ∈O g.
+Proof.
+  intros (c1&n1&H1).
+  eexists (c1*c), (n1).
+  intros.
+  rewrite H1.
+  all:Lia.lia.
+Qed.
+
+Lemma inO_mul_c_r c f1  g:
+  f1 ∈O g -> (fun n => f1 n * c) ∈O g.
+Proof.
+  intros (c1&n1&H1).
+  eexists (c1*c),(n1).
+  intros.
+  rewrite H1.
+  all:Lia.lia.
+Qed.
+
+
+Lemma inO_c c f':
+  (fun _ => 1) ∈O f' ->  
+  (fun _ => c ) ∈O f'.
+Proof.
+  intros H'.
+  assert (H:c<= 1*c) by lia.
+  setoid_rewrite H. eapply inO_mul_c_r. easy.
+Qed.
+(*
+Lemma inO_c c n0 f':
+  (forall n', n0 <= n' -> 1 <= f' n') ->  
+  (fun _ => c ) ∈O f'.
+Proof.
+  eexists (c),(n0).
+  intros. rewrite <- H. all:Lia.nia.
+Qed. *)
+
+Lemma inO_leq n0 f' g:
+  (forall n', n0 <= n' -> f' n' <= g n') ->  
+  f' ∈O g.
+Proof.
+  eexists 1,(n0).
+  intros. rewrite <- H. all:Lia.nia.
+Qed.
+
+Smpl Create inO.
+
+Smpl Add 11 (smpl monotonic) : inO.
+
+Smpl Add 10 (first [ simple eapply inO_add_l | simple eapply inO_mul_c_l | simple eapply inO_mul_c_r | progress (eapply inO_c) | reflexivity]) (*
+                    | simple eapply inO_c with (n0:=1);intro;try rewrite <- !f_geq_n;Lia.nia
+                                 | inO_leq 1])*) : inO.
+
+Ltac smpl_inO := repeat (smpl inO).
+
+Lemma inO_mul_l f1 f2  g1 g2:
+  f1 ∈O g1 -> f2 ∈O g2 -> (fun n => f1 n * f2 n) ∈O (fun n => g1 n * g2 n).
+Proof.
+  intros (c1&n1&H1) (c2&n2&H2).
+  eexists (c1 * c2),(max n1 n2).
+  intros.
+  rewrite H1,H2.
+  all:Lia.lia.
+Qed.
+
+Lemma inO_comp_l f1 f2  g1 g2:
+  f1 ∈O g1 -> f2 ∈O g2 ->
+  monotonic f1 ->
+  (forall x, x <= g2 x ) ->
+  (forall c, (fun x => g1 (c*x)) ∈O g1) -> (fun n => f1 (f2 n)) ∈O (fun n => g1 (g2 n)).
+Proof.
+  intros (c1&n1&H1) (c2&n2&H2) mono2 H' H.
+  specialize (H (c2+n1)) as (c2'&n2'&H).
+  eexists (c1 * c2'),(max (max 1 n2') n2).
+  intros.
+  etransitivity.
+  {hnf in mono2. rewrite mono2. reflexivity. transitivity ((c2+n1)*(g2 n)). 2:reflexivity. rewrite H2. Lia.nia. lia. }
+  specialize (H' n).
+  setoid_rewrite H1. 2:Lia.nia.
+  rewrite H. Lia.nia. Lia.nia.
+Qed.
+
+
+
+Lemma inO__bound f g (H:f ∈O g) : exists c, forall n, f n <= c + c * g n.
+Proof.
+  destruct H as (c0&n0&H). cbn.
+  exists (max c0 (maxl (map f (natsLess n0)))).
+  intros n.
+  decide (n0<=n).
+  -rewrite H. all:Lia.nia.
+  -rewrite (@maxl_leq (f n) (map f (natsLess n0))). Lia.nia. apply in_map_iff. setoid_rewrite natsLess_in_iff. exists n. intuition.
+Qed.
+
+(** *** smallO *)
+
+(** This variant of smallo does not need real nubers, as we moved the constant to the other side *)
+Definition ino (f g : nat -> nat) : Prop := forall c__inv, exists n0 , forall n, n0 <= n -> c__inv * f n < g n.
+
+Notation " f ∈o g" := (ino f g) (at level 70).
+
+(*Definition n__ino f g (H:f ∈o g) c0 (H' : 0 < c0) : nat := proj1_sig (ino__correct H c0 H').
+
+Definition correct_n__ino f g (H:f ∈o g) c0 (H' : 0 < c0)
+  : forall n, n__ino H H' <= n -> f n < c0 * g n := proj2_sig (ino__correct H c0 H').
+ *)
+
+Lemma ino_inO_incl f g :
+  f ∈o g -> f ∈O g.
+Proof.
+  intros H.
+  specialize (H 1) as (c__ino&H).
+  exists 1,c__ino. intros ? ?%H. lia.
+Qed.
+
+
+(** ** O(poly)*)
+
+Definition inOPoly (f : nat -> nat) : Prop :=
+  exists n, f ∈O (fun x => x ^ n).
+
+
+Lemma inOPoly_c c: inOPoly (fun _ => c).
+Proof.
+  exists 1. eapply inO_c. cbn. eapply (inO_leq (n0:=1)). intros. lia.
+Qed.
+
+Lemma inOPoly_x: inOPoly (fun x => x).
+Proof.
+  exists 1. cbn. eapply (inO_leq (n0:=1)). intros. lia.
+Qed.
+
+Lemma inOPoly_add f1 f2: inOPoly f1 -> inOPoly f2 -> inOPoly (fun x => f1 x + f2 x).
+Proof.
+  intros (n1&?) (n2&?).
+  exists (max n1 n2). 
+  eapply inO_add_l.
+  all:etransitivity;[eassumption|].
+  all:eapply inO_leq with (n0:=1).
+  all:intros ? ?.
+  all:eapply Nat.pow_le_mono_r. all:Lia.nia.
+Qed.
+
+Lemma inOPoly_mul f1 f2: inOPoly f1 -> inOPoly f2 -> inOPoly (fun x => f1 x * f2 x).
+Proof.
+  intros (n1&?) (n2&?).
+  exists (n1+n2). 
+  transitivity (fun x : nat => x ^ n1 * x^n2).
+  1:now eauto using inO_mul_l.
+  all:eapply inO_leq with (n0:=0).
+  all:intros ? _.
+  rewrite Nat.pow_add_r. Lia.nia.
+Qed.
+
+Lemma inOPoly_comp f1 f2: monotonic f1 -> inOPoly f1 -> inOPoly f2 -> inOPoly (fun x => f1 (f2 x)).
+Proof.
+  intros ? (n1&?) (n2&?).
+  exists ((max 1 n2)*n1). 
+  etransitivity.
+  {eapply inO_comp_l with (g2:=(fun x => x ^(max 1 n2))).
+   1,3:eassumption.
+   -rewrite H1. apply inO_leq with (n0:=1). intros.
+    eapply Nat.pow_le_mono;lia.
+   -intros. replace x with (x^1) at 1 by (cbn;Lia.nia).
+    decide (x=0). 2:now eapply Nat.pow_le_mono;Lia.nia.
+    subst x. rewrite !Nat.pow_0_l. all:Lia.nia.
+   -cbn beta. intros c.
+    exists (c^n1),0. intros.
+    rewrite Nat.pow_mul_l. reflexivity.
+  }
+  cbn beta.
+  eapply inO_leq with (n0:=0). intros.
+  rewrite Nat.pow_mul_r. reflexivity.
+Qed.
+
+Smpl Add 10 (first [ simple eapply inOPoly_add | simple eapply inOPoly_mul | simple eapply inOPoly_c | simple eapply inOPoly_x | eassumption])  : inO.
+
+
+Instance inO_inOPoly_trans : Proper (Basics.flip inO ==> Basics.impl) inOPoly.
+Proof.
+  intros ? ? ? [? R2]. unfold inOPoly. eexists. setoid_rewrite <- R2. easy.
+Qed.
