theories/L/Complexity/Problems/TMGenericNPcompleteProblem.v
@@ -1,0 +1,65 @@
+From Undecidability.TM Require Import TM.
+From Undecidability.L.TM Require Import TMflatEnc TMEncoding TapeDecode.
+From Undecidability.L.Datatypes Require Import LNat LProd Lists.
+
+
+(*** TODO: move M
+  or parts of initial tape into definition? **)
+
+Definition TMgenericNPcompleteProblem: TM*nat*nat -> Prop:=
+  fun '(M,maxSize, steps (*in unary*)) =>
+    exists sig n (M':mTM sig n), M ∼ M' /\ (exists t, (exists f, loopM (initc M' t) steps = Some f
+               /\ TM.halt (cstate f) = true)
+         /\ sizeOfmTapes t <= maxSize).
+
+
+From Undecidability.L.Complexity Require Import NP LinTimeDecodable.
+From Undecidability.L Require Import Tactics.LTactics Functions.Decoding TMflatFun.
+
+
+
+Lemma inNP_TMgenericNPCompleteProblem:
+  inNP TMgenericNPcompleteProblem.
+Proof.
+  apply inNP_intro with (R:= fun '(M,maxSize, steps (*in unary*)) t =>
+                                exists sig n (M':mTM sig n) t', isFlatteningTapesOf t t' /\ M ∼ M' 
+                                       /\ (exists f, loopM (initc M' t') steps = Some f
+                                       /\ TM.halt (cstate f) = true)
+                                       /\ sizeOfmTapes t' <= maxSize).
+  now apply linDec_polyTimeComputable.
+  -evar (f':nat -> nat).
+   exists f'. repeat eapply conj.
+   {
+     eexists (fun '((M,maxSize,steps),t) => _). repeat eapply conj.
+     2:{intros [[[TM maxSize] steps] y].  cbn. admit.
+     }
+     all:admit.
+   }
+   all:admit.
+  -evar (f:nat -> nat).
+   exists f. repeat eapply conj.
+   2:{
+     intros [[TM maxSize] steps] y.
+     intros (?&?&?&?&R__tapes&?&?).
+     remember (size (enc (TM, maxSize, steps))) as n eqn:Hn.
+     rewrite size_flatTapes. 2:eassumption.
+     rewrite !size_prod,size_TM in Hn.
+     destruct TM;cbn [fst snd] in Hn.
+     destruct H;cbn in *. subst x0.
+     unshelve erewrite ((_ : tapes <= n)) at 1 3.
+     {rewrite size_nat_enc with (n:=tapes) in Hn. lia. }
+     unshelve erewrite ((_ : sizeOfmTapes x2 <= n)) at 1 3.
+     {rewrite size_nat_enc with (n:=maxSize) in Hn. lia. }
+     unshelve erewrite ((_ : Cardinality.Cardinality x <= n)) at 1.
+     {rewrite size_nat_enc with (n:=sig) in Hn. lia. }
+     [f]:intros s. unfold f. reflexivity.
+   }
+   all:unfold f;smpl_inO.
+  -unfold TMgenericNPcompleteProblem.
+   intros [[] ].
+   
+   setoid_rewrite isFlatteningTapesOf_iff.
+   split.
+   +intros (?&?&?&?&?&?&?). eauto 10.
+   +intros (?&?&?&?&?&?&?&?&?). eauto 10.
+Admitted.
