theories/L/Complexity/RegisteredP.v
@@ -1,0 +1,127 @@
+From Undecidability.L.Tactics Require Import LTactics.
+From Undecidability.L.Datatypes Require Import LProd LTerm.
+
+From Undecidability.L Require Import Complexity.Synthetic Complexity.Monotonic Functions.Encoding TM.TMEncoding.
+
+Class registeredP `(X:Type) `{registered X}: Type :=
+  {
+    c__regP : nat;
+    comp_enc_lin : computableTime' (enc (X:=X)) (fun x _ => (size (enc x) *c__regP,tt));
+  }.
+
+Arguments registeredP : clear implicits.
+Arguments registeredP _ {_}.
+Arguments c__regP : clear implicits.
+Arguments c__regP _ {_ _} : simpl never.
+Hint Mode registeredP + + : typeclass_instances. (* treat argument as input and force evar-freeness*)
+
+Existing Instance comp_enc_lin.
+Global Typeclasses Opaque enc.
+
+
+Instance regP_nat : registeredP nat.
+Proof.
+  evar (c:nat).
+  exists c.
+  eexists _. 
+  eapply computesTime_timeLeq.
+  2:now apply term_nat_enc.
+  repeat intro. split. 2:easy.
+  cbn [fst]. rewrite -> size_nat_enc. [c]:exact 4. unfold c. nia.
+Qed.
+
+
+Instance regP_term : registeredP term.
+Proof.
+  evar (c:nat).
+  exists c.
+  eexists _. 
+  eapply computesTime_timeLeq.
+  2:now apply term_term_enc.
+  repeat intro. split. 2:easy.
+  cbn [fst]. rewrite -> size_term_enc_r. [c]:exact 30. unfold c. nia.
+Qed.
+
+Instance regP_Prod X Y `{registeredP X} `{registeredP Y}: registeredP (X*Y).
+Proof.
+  evar (c:nat).
+  exists c.
+  eexists _. 
+  eapply computesTime_timeLeq.
+  2:now apply term_prod_enc.
+  intros [] _. split. 2:easy.
+  cbn [fst]. rewrite -> size_prod.
+  cbn. [c]:exact (c__regP X + c__regP Y + 4). unfold c. nia.
+Qed.
+
+Import Lists.
+
+Instance regP_list X `{registeredP X}: registeredP (list X).
+Proof.
+  evar (c:nat).
+  exists c.
+  eexists _. 
+  eapply computesTime_timeLeq.
+  2:now apply term_list_enc.
+  intros l _. split. 2:easy.
+  cbn [fst]. rewrite -> size_list.
+  cbn. [c]:exact (c__regP X + 4). unfold c.
+  induction l;cbn. all:nia.
+Qed.
+
+Import LOptions.
+
+Instance regP_option X `{registeredP X}: registeredP (option X).
+Proof.
+  evar (c:nat).
+  exists c.
+  eexists _. 
+  eapply computesTime_timeLeq.
+  2:now apply term_option_enc.
+  intros l _. split. 2:easy.
+  cbn [fst]. rewrite -> size_option.
+  [c]:exact (c__regP X + 5). unfold c.
+  now destruct l.
+Qed.
+
+
+Instance term_move_enc
+  :computableTime' (TMEncoding.move_enc) (fun x _ => (15,tt)).
+Proof.
+  extract. solverec.
+Qed.
+
+Instance term_bool_enc
+  :computableTime' (LBool.bool_enc) (fun x _ => (12,tt)).
+Proof.
+  extract. solverec.
+Qed.
+
+
+Instance regP_move : registeredP TM.move.
+Proof.
+  evar (c:nat).
+  exists c.
+  eexists _. 
+  eapply computesTime_timeLeq.
+  2:now apply term_move_enc.
+  intros l _. split. 2:easy.
+  change (enc l) with (TMEncoding.move_enc l).
+  cbn.
+  [c]:exact (4). unfold c.
+  destruct l;cbn [size TMEncoding.move_enc]. all:lia.
+Qed.
+
+Instance regP_bool : registeredP bool.
+Proof.
+  evar (c:nat).
+  exists c.
+  eexists _. 
+  eapply computesTime_timeLeq.
+  2:now apply term_bool_enc.
+  intros l _. split. 2:easy.
+  change (enc l) with (LBool.bool_enc l).
+  cbn.
+  [c]:exact (4). unfold c.
+  destruct l;cbn [size LBool.bool_enc]. all:lia.
+Qed.
