theories/L/TM/TMflatEnc.v
@@ -1,0 +1,138 @@
+From Undecidability.L.Tactics Require Import LTactics GenEncode.
+From Undecidability.L.Datatypes Require Import LNat Lists LProd LOptions .
+From Undecidability.L Require Import Functions.Decoding.
+
+
+From Undecidability.L.TM Require Export TMflat.
+From Undecidability.L.TM Require Import TMEncoding.
+
+
+Run TemplateProgram (tmGenEncode "TM_enc" TM).
+Hint Resolve TM_enc_correct : Lrewrite.
+
+
+Instance term_Build_TM : computableTime' (Build_TM) (fun _ _ => (1,fun _ _ => (1,fun _ _ => (1,fun _ _ => (1,fun _ _ => (1,fun _ _ => (1,tt))))))).
+Proof.
+  extract constructor. solverec. 
+Defined.
+
+Instance term_sig : computableTime' sig (fun _ _ => (9,tt)).
+Proof.
+  extract. solverec.
+Defined.
+
+
+Instance term_tapes : computableTime' tapes (fun _ _ => (9,tt)).
+Proof.
+  extract. solverec.
+Defined.
+
+Instance term_states : computableTime' states (fun _ _ => (9,tt)).
+Proof.
+  extract. solverec.
+Defined.
+
+Instance term_trans : computableTime' trans (fun _ _ => (9,tt)).
+Proof.
+  extract. solverec.
+Defined.
+
+Instance term_start : computableTime' start (fun _ _ => (9,tt)).
+Proof.
+  extract. solverec.
+Defined.
+
+Instance term_halt : computableTime' halt (fun _ _ => (9,tt)).
+Proof.
+  extract. solverec.
+Defined.
+
+
+(*
+Definition TM_decode (s : term) : option TM :=
+  match s with
+  | lam (app(app(app(app(app (app O sig) tapes) states) trans) start) halt) =>
+    match decode nat sig,decode nat tapes, decode nat states, decode (list (nat * list (option nat) * (nat * list (option nat * TM.move)))) trans, decode nat start, decode (list bool) halt with
+      Some sig, Some tapes, Some states, Some trans, Some start, Some halt =>
+      Some (Build_TM sig tapes states trans start halt)
+    | _,_,_,_,_,_ => None
+    end
+  | _ => None
+  end.
+
+Arguments list_decode : clear implicits.
+Arguments list_decode _ {_ _} _.
+
+Instance decode_TM : decodable TM.
+Proof.
+  exists (list_decode X).
+  all:unfold enc at 1. all:cbn.
+  -induction x;cbn.
+   +easy.
+   +setoid_rewrite decode_correct. now rewrite IHx.
+  -apply (size_induction (f := size) (p := (fun t => forall x, list_decode X t = Some x -> list_enc x = t))). intros t IHt s.
+   destruct t eqn:eq. all:cbn.
+   all:repeat let eq := fresh in destruct _ eqn:eq. all:try congruence.
+   all:intros [= <-].
+   +easy.
+   +cbn. change (match H with
+                | @mk_registered _ enc _ _ => enc
+                 end x) with (enc x). erewrite decode_correct2. 2:easy.
+    erewrite IHt.
+    *reflexivity.
+    *cbn;lia.
+    *easy.
+Defined.
+
+
+Instance linDec_TM : linTimeDecodable TM.
+Proof.
+  exists c__encTM.
+  eexists _. 
+  eapply computesTime_timeLeq.
+  2:now apply term_TM_enc.
+  intros l _. split. 2:easy.
+  cbn [fst]. reflexivity.
+Qed.
+
+*)
+
+Lemma size_TM (M:TM):
+  size (enc M) = let (a,b,c,d,e,f) := M in size (enc a) + size (enc b) +size (enc c) +size (enc d) + size (enc e) + size (enc f) + 8.
+Proof.
+  change (enc M) with (TM_enc M).
+  destruct M as []. cbn. solverec.
+Qed.
+
+From Undecidability.L.Complexity Require Export RegisteredP LinTimeDecodable.
+
+
+Definition c__encTM := max (c__regP (list (nat * list (option nat) * (nat * list (option nat * TM.move))))) (max (c__regP nat) (max (c__regP (list bool)) 4)).
+
+Instance term_TM_enc
+  :computableTime' (TM_enc) (fun x _ => (size (enc x) * c__encTM,tt)).
+Proof.
+  unfold TM_enc.
+  change (@list_enc (nat * list (option nat) * (nat * list (option nat * TM.move))) _) with (enc (X:=list (nat * list (option nat) * (nat * list (option nat * TM.move))))).
+  change (@list_enc bool _) with (enc (X:=list bool)).
+  change (nat_enc) with (enc (X:=nat)).
+  extract.
+  intros _ M [].
+  rewrite size_TM.
+  recRel_prettify2.
+  repeat (lazymatch goal with |- context C[@size ?a] => generalize (@size a);intro end).
+  assert (H':c__encTM <= c__encTM) by easy.
+  repeat setoid_rewrite Nat.max_lub_iff in H'.
+  destruct H' as (H1&H2&H3&H4).
+  repeat rewrite H1. repeat rewrite H2. repeat rewrite H3. rewrite <- H4 at 13. lia.
+Qed.
+
+Instance regP_TM : registeredP TM.
+Proof.
+  exists c__encTM.
+  eexists _. 
+  eapply computesTime_timeLeq.
+  2:now apply term_TM_enc.
+  intros l _. split. 2:easy.
+  cbn [fst]. reflexivity.
+Qed.
