theories/L/TM/TapeDecode.v
@@ -1,0 +1,18 @@
+From Undecidability.L.Tactics Require Import LTactics GenEncode.
+From Undecidability.L.Datatypes Require Import LNat Lists LProd LFinType.
+From Undecidability.L Require Import TM.TMEncoding.
+
+
+From Undecidability Require Import TM.TM.
+
+From Undecidability.L Require Import Functions.Decoding Complexity.Synthetic Complexity.LinTimeDecodable.
+
+Instance linDec_tape X `{_:linTimeDecodable X}: linTimeDecodable (tape X).
+Proof.
+  evar (c:nat). exists c.
+  unfold decode, decode_tape,tape_decode.
+  extract.
+  recRel_prettify2;cbn[size];ring_simplify. idtac. 
+  [c]:exact (max (c__linDec (list X)) (max (c__linDec (X)) 11)).
+  all:unfold c;try nia.
+Qed.
